src/PlutusIR/Transform/DeadCode/Decide2.v
@@ -1,0 +1,64 @@
+Require Import
+  Lists.List
+  Strings.String
+.
+From PlutusCert Require Import
+  Util
+  PlutusIR
+  PlutusIR.Analysis.Equality
+  DeadCode2
+  Compat
+  Purity
+  Size
+  Analysis.BoundVars
+.
+
+Import NamedTerm.
+Import ListNotations.
+
+Require Import
+  Arith.
+
+Section Bindings.
+
+  Context (dec_Term : Term -> Term -> bool).
+
+  Definition dec_Binding (b b' : Binding) : bool := match b, b' with
+    | TermBind s vd t, TermBind s' vd' t' => Strictness_eqb s s' && VDecl_eqb vd vd' && dec_Term t t'
+    | b, b' => Binding_eqb b b'
+    end.
+
+  Definition unused_in (b : Binding) (t' : Term) : bool :=
+    forallb (fun x => negb (existsb (String.eqb x) (fv t'))) (bvb b) &&
+    forallb (fun x => negb (existsb (String.eqb x) (ftv t'))) (btvb b)
+  .
+
+  (* t' is the post-term let body *)
+  Fixpoint dec_Bindings_NonRec (bs bs' : list Binding) (t' : Term) : bool :=
+    match bs, bs' with
+    | b :: bs, b' :: bs' =>
+        if dec_Binding b b'
+        then dec_Bindings_NonRec bs bs' t'
+        else
+          dec_pure_binding [] b &&
+          unused_in b (Let NonRec bs' t') &&
+          dec_Bindings_NonRec bs (b' :: bs') t'
+    | [], [] => true
+    | b :: bs, [] =>
+          dec_pure_binding [] b &&
+          unused_in b t' &&
+          dec_Bindings_NonRec bs [] t'
+    | [], _ => (* Left-over bindings in post-term, impossible *)
+        false
+    end.
+
+End Bindings.
+
+Fixpoint dec_Term (t t' : Term) {struct t} :=
+  match t, t' with
+  | Let NonRec bs t, Let NonRec bs' t' =>
+      if dec_Bindings_NonRec dec_Term bs bs' t'
+      then dec_Term t t'
+      else false
+  | _, _ => dec_compat dec_Term t t'
+  end.
