src/PlutusIR/Transform/DeadCode/Intermediate.v
@@ -1,0 +1,130 @@
+Require Import
+  Lists.List
+  Strings.String
+.
+From PlutusCert Require Import
+  Util
+  PlutusIR
+  PlutusIR.Analysis.Equality
+  DeadCode2
+  Compat
+  Purity
+  Size
+  Analysis.BoundVars
+.
+
+Import NamedTerm.
+Import ListNotations.
+
+Require Import 
+  Arith.
+
+
+Section Bindings.
+  Context (mk : Term -> Term -> option Term).
+
+  Definition mk_Binding  (b b' : Binding) : option Binding :=
+    match b, b' with
+      | TermBind s vd t, TermBind s' vd' t' =>
+          if Strictness_eqb s s' &&
+            VDecl_eqb vd vd'
+          then TermBind s vd <$> mk t t'
+          else None
+      | DatatypeBind dtd, DatatypeBind dtd' =>
+          if DTDecl_eqb dtd dtd'
+            then pure (DatatypeBind dtd)
+            else None
+      | TypeBind tvd ty, TypeBind tvd' ty' =>
+          if TVDecl_eqb tvd tvd' &&
+            Ty_eqb ty ty'
+          then pure (TypeBind tvd ty)
+          else None
+      | _, _ => None
+    end
+  .
+
+  Fixpoint match_Bindings
+    (bs bs' : list Binding)
+    : bool :=
+      match bs, bs' with
+
+      | b :: bs, b' :: bs' =>
+          match mk_Binding b b' with
+          | None => (* Binding was removed *)
+              match_Bindings bs (b' :: bs')
+          | Some _ => (* Binding matches *)
+              match_Bindings bs bs'
+          end
+      | _ , [] => (* All were removed *)
+          true
+      | [] , _ :: _ => (* Some bindings that didn't exist: the whole block in the pre-term was removed *)
+          false
+      end
+  .
+  End Bindings.
+
+  Fixpoint mk (t t' : Term) {struct t} : option Term :=
+    match t, t' with
+    | Let rec bs t
+    , Let rec' bs' t' =>
+        if Recursivity_eqb rec rec'
+          then
+            if match_Bindings mk bs bs'
+              then Let rec bs' <$> mk t t'
+              else
+                (* Whole let block was removed *)
+                Let rec [] <$> mk t t'
+          else
+            (* Whole let block was removed *)
+            Let rec [] <$> mk t t'
+    | Let rec bs t
+    , t' => (* Whole block was removed *)
+        Let rec [] <$> mk t t'
+    | LamAbs n ty t
+    , LamAbs n' ty' t' =>
+        if String.eqb n n' &&
+          Ty_eqb ty ty'
+        then LamAbs n ty <$> mk t t'
+        else None
+    | Var n, Var n' =>
+        if String.eqb n n'
+          then Some (Var n)
+          else None
+    | TyAbs n k t, TyAbs n' k' t' =>
+        if String.eqb n n' &&
+           Kind_eqb k k'
+        then TyAbs n k <$> mk t t'
+        else None
+    | Apply s t, Apply s' t' =>
+        Apply <$> mk s s' <*> mk t t'
+    | TyInst t ty, TyInst t' ty' =>
+        if Ty_eqb ty ty'
+        then TyInst <$> (mk t t') <*> pure ty
+        else None
+    | IWrap ty1 ty2 t, IWrap ty1' ty2' t' =>
+        if Ty_eqb ty1 ty1' &&
+           Ty_eqb ty2 ty2'
+        then IWrap ty1 ty2 <$> mk t t'
+        else None
+    | Unwrap t, Unwrap t' =>
+        Unwrap <$> mk t t'
+    | Error ty, Error ty' =>
+        if Ty_eqb ty ty'
+          then pure (Error ty)
+          else None
+    | Constant v, Constant v' =>
+        if some_valueOf_eqb v v'
+          then pure (Constant v)
+          else None
+    | Builtin f, Builtin f' =>
+        if func_eqb f f'
+          then pure (Builtin f)
+          else None
+    | Constr i ts, Constr i' ts' => 
+        if Nat.eqb i i'
+          then Constr i <$> sequence_options (zip_with mk ts ts')
+          else None
+    | Case t ts, Case t' ts' =>
+          Case <$> mk t t' <*> sequence_options (zip_with mk ts ts')
+    | _, _ => None
+   end.
